theories/Interaction_Between_Lts/Examples_of_Interactions/ForwarderConstruction.v
@@ -38,9 +38,9 @@ From Must Require Import MultisetHelper gLts Bisimulation Lts_OBA Lts_FW Lts_OBA
 
 Definition fw_inter `{ExtAction A} μ2 μ1 := dual μ2 μ1 /\ non_blocking μ1.
 
-#[global] Program Instance FW_gLts {P A : Type} `{H : ExtAction A} (M: gLts P A) 
-  `{@Prop_of_Inter P (mb A) A fw_inter H M MbgLts}
-    : gLts (P * mb A) A := inter_lts fw_inter.
+#[global] Program Instance FW_gLts {P A : Type} `(M: gLts P A) 
+  {_ : Prop_of_Inter P (mb A) A fw_inter}
+    : gLts (P * mb A) _ := inter_lts fw_inter.
 
 (* Properties on the Forwarder Construction *)
 
@@ -149,7 +149,7 @@ Proof.
 Qed.
 
 Definition lts_fw_sc
-  `{M1 : @gLtsOba P A H gLtsP gLtsEqP}
+  `{M1 : @gLtsOba P A H gLtsEqP}
   `{@Prop_of_Inter P (mb A) A fw_inter H gLtsP MbgLts}
   (p : P * mb A) α (q : P * mb A) :=
   exists r, ((FW_gLts gLtsP).(lts_step) p α r) /\ r ≐ q.
@@ -198,23 +198,23 @@ Proof.
   - multiset_solver.
 Qed.
 
-Lemma lts_fw_eq_spec_left_blocking_action `{
-   M : @gLtsObaFB P A H gLtsP gLtsEqP gLtsObaP}
-   `{@Prop_of_Inter P (mb A) A fw_inter H gLtsP MbgLts}
+Lemma lts_fw_eq_spec_left_blocking_action 
+  `{M : @gLtsObaFB P A H gLtsEqP gLtsObaP}
+   `{!Prop_of_Inter P (mb A) A fw_inter}
    p q q' mp mq β :
    p ▷ mp ≐ q ▷ mq -> blocking β -> q ⟶[β] q'
     -> p ▷ mp ⟶≐[β] q' ▷ mq.
 Proof.
-  intros not_nb heq l.
+  intros not_nb heq l. unfold gLtsEq_gLts in l.
   edestruct (fw_eq_blocking_action_simulation not_nb heq l) as (p' & hl' & heq').
   exists (p' ▷ mp). split.
   + eapply ParLeft. eauto with mdb.
   + eauto with mdb.
 Qed.
 
-Lemma lts_fw_eq_spec_left_non_blocking_action `{
-  M : @gLtsObaFB P A H gLtsP gLtsEqP gLtsObaP}
-  `{@Prop_of_Inter P (mb A) A fw_inter H gLtsP MbgLts}
+Lemma lts_fw_eq_spec_left_non_blocking_action
+  `{M : @gLtsObaFB P A H gLtsEqP gLtsObaP}
+   `{!Prop_of_Inter P (mb A) A fw_inter}
   p q q' mp mq η :
   p ▷ mp ≐ q ▷ mq -> non_blocking η -> q ⟶[η] q' -> p ▷ mp ⟶≐[η] q' ▷ mq.
 Proof.
@@ -274,8 +274,8 @@ Proof.
 Qed.
 
 Lemma lts_fw_eq_spec_left_tau
-  `{M : @gLtsObaFB P A H gLtsP gLtsEqP gLtsObaP}
-  `{@Prop_of_Inter P (mb A) A fw_inter H gLtsP MbgLts}
+  `{M : @gLtsObaFB P A H gLtsEqP gLtsObaP}
+   `{!Prop_of_Inter P (mb A) A fw_inter}
   (p : P) (q : P) q' (mp : mb A) (mq : mb A) :
   p ▷ mp ≐ q ▷ mq -> q ⟶ q'
     -> p ▷ mp ⟶≐ q' ▷ mq.
@@ -390,9 +390,9 @@ Proof.
     + multiset_solver.
 Qed.
 
-Lemma lts_fw_eq_spec_left `{
-  M : @gLtsObaFB P A H gLtsP gLtsEqP gLtsObaP}
-  `{@Prop_of_Inter P (mb A) A fw_inter H gLtsP MbgLts}
+Lemma lts_fw_eq_spec_left
+  `{M : @gLtsObaFB P A H gLtsEqP gLtsObaP}
+   `{!Prop_of_Inter P (mb A) A fw_inter}
   p q q' α mp mq :
   p ▷ mp ≐ q ▷ mq -> q ⟶{α} q'
     -> p ▷ mp ⟶≐{α} q' ▷ mq.
@@ -404,9 +404,9 @@ Proof.
   + eapply lts_fw_eq_spec_left_tau; eauto.
 Qed.
 
-Lemma lts_fw_eq_spec_right_non_blocking_action `{
-  M : @gLtsObaFB P A H gLtsP gLtsEqP gLtsObaP}
-  `{@Prop_of_Inter P (mb A) A fw_inter H gLtsP MbgLts}
+Lemma lts_fw_eq_spec_right_non_blocking_action 
+  `{M : @gLtsObaFB P A H gLtsEqP gLtsObaP}
+   `{!Prop_of_Inter P (mb A) A fw_inter}
   p q mp mq η :
   non_blocking η -> p ▷ mp ≐ q ▷ {[+ η +]} ⊎ mq
     -> p ▷ mp ⟶≐[η] q ▷ mq.
@@ -464,9 +464,9 @@ Proof.
     now rewrite gmultiset_disj_union_comm.
 Qed.
 
-Lemma lts_fw_eq_spec_right_blocking_action `{
-  M : @gLtsObaFB P A H gLtsP gLtsEqP gLtsObaP}
-  `{@Prop_of_Inter P (mb A) A fw_inter H gLtsP MbgLts}
+Lemma lts_fw_eq_spec_right_blocking_action 
+  `{M : @gLtsObaFB P A H gLtsEqP gLtsObaP}
+   `{!Prop_of_Inter P (mb A) A fw_inter}
    p q mp mq η μ:
   non_blocking η -> dual μ η -> p ▷ mp ≐ q ▷ mq 
     -> p ▷ mp ⟶≐[μ] q ▷ {[+ η +]} ⊎ mq.
@@ -482,9 +482,9 @@ Proof.
       rewrite (lts_mb_nb_spec1 η mq nb). multiset_solver.
 Qed.
 
-Lemma lts_fw_com_eq_spec `{
-  M : @gLtsObaFB P A H gLtsP gLtsEqP gLtsObaP}
-  `{@Prop_of_Inter P (mb A) A fw_inter H gLtsP MbgLts}
+Lemma lts_fw_com_eq_spec 
+  `{M : @gLtsObaFB P A H gLtsEqP gLtsObaP}
+   `{!Prop_of_Inter P (mb A) A fw_inter}
   p q q' mp mq β η:
   blocking β -> dual β η -> non_blocking η -> p ▷ mp ≐ q ▷ {[+ η +]} ⊎ mq -> q ⟶[β] q' 
     -> p ▷ mp ⟶≐ q' ▷ mq.
@@ -518,8 +518,8 @@ Proof.
          eapply strip_eq_step in hsph' as h1; eauto.
          destruct h1 as (p4 & hsu & heqp4).
          symmetry. transitivity ph'. now symmetry. transitivity p4. now symmetry.
-         eapply (@strip_eq_sim _ _ _ _ _ _ p2' p3). transitivity p2. assumption. now symmetry.
-         eassumption.
+         eapply (strip_eq_sim (p := p2') (q := p3)). 
+         transitivity p2.  assumption. now symmetry. eassumption.
          replace (lts_oba_mo p' ∖ {[+ η +]}) with (lts_oba_mo p3). assumption.
          rewrite <- heqmu. eapply lts_oba_mo_eq. transitivity p2. assumption. now symmetry.
       ++ eapply (gmultiset_disj_union_inj_1 {[+ η +]}).
@@ -559,9 +559,9 @@ Proof.
     multiset_solver.
 Qed.
 
-Lemma lts_fw_eq_spec  `{
-  M : @gLtsObaFB P A H gLtsP gLtsEqP gLtsObaP}
-  `{@Prop_of_Inter P (mb A) A fw_inter H gLtsP MbgLts}
+Lemma lts_fw_eq_spec  
+  `{M : @gLtsObaFB P A H gLtsEqP gLtsObaP}
+   `{!Prop_of_Inter P (mb A) A fw_inter}
   (p : P) (q : P) (t : P) (mp : mb A) (mq : mb A) (mt : mb A) (α : Act A) :
   (p ▷ mp) ≐ (t ▷ mt) -> (t ▷ mt) ⟶{α} (q ▷ mq)
     -> p ▷ mp ⟶≐{α} q ▷ mq.
@@ -587,9 +587,9 @@ Qed.
 (* Our FW Equivalence ≐ is a bissimulation *)
 
 #[global] Program Instance FW_gLtsEq 
-  `{M : @gLtsObaFB P A H gLtsP gLtsEqP gLtsObaP}  
-  `{@Prop_of_Inter P (mb A) A fw_inter H gLtsP MbgLts}
-  : gLtsEq (P * mb A) A :=
+  `{M : @gLtsObaFB P A H gLtsEqP gLtsObaP}
+   `{!Prop_of_Inter P (mb A) A fw_inter}
+  : gLtsEq (P * mb A) _ :=
   {| eq_rel := fw_eq |}.
 Next Obligation. intros. split.
   + eapply fw_eq_refl.
@@ -597,17 +597,17 @@ Next Obligation. intros. split.
   + eapply fw_eq_trans.
 Qed.
 Next Obligation.
-  intros ? ? ? ? ? ? ? ? (p, mp) (q, mq) α ((t, mt) & heq & hl).
+  intros ? ? ? ? ? ? ? (p, mp) (q, mq) α ((t, mt) & heq & hl).
   eapply lts_fw_eq_spec; eauto.
 Qed.
 
 #[global] Program Instance FW_gLtsOba
-  `{M : @gLtsObaFB P A H gLtsP gLtsEqP gLtsObaP}  
-  `{@Prop_of_Inter P (mb A) A fw_inter H gLtsP MbgLts}
-  : gLtsOba (P * mb A) A :=
+  `{M : @gLtsObaFB P A H gLtsEqP gLtsObaP}
+   `{!Prop_of_Inter P (mb A) A fw_inter}
+  : gLtsOba (P * mb A) :=
   {| lts_oba_mo p := lts_oba_mo p.1 ⊎ mb_without_not_nb p.2 |}.
 Next Obligation.
-  intros ? ? ? ? ? ? ? ? p1 η p2 nb Hstep; simpl in *.
+  intros ? ? ? ? ? ? ? p1 η p2 nb Hstep; simpl in *.
   inversion Hstep; subst; simpl in *.
   + apply (lts_oba_mo_spec_bis1 a1 η a2) in nb; eauto. set_solver.
   + apply (non_blocking_action_in_ms b1 η b2) in nb as eq ; subst;  eauto. 
@@ -616,7 +616,7 @@ Next Obligation.
     set_solver.
 Qed.
 Next Obligation.
-  intros ? ? ? ? ? ? ? ? (p , mem) η mem_non_blocking; simpl in *.
+  intros ? ? ? ? ? ? ? (p , mem) η mem_non_blocking; simpl in *.
   rewrite gmultiset_elem_of_disj_union in mem_non_blocking. 
   destruct (decide (η ∈ lts_oba_mo p)) as [non_blocking_in_p | non_blocking_not_in_p].
   + eapply lts_oba_mo_spec_bis2 in non_blocking_in_p as (p' & nb & Hstep).
@@ -632,7 +632,7 @@ Next Obligation.
     * exfalso. destruct mem_non_blocking; contradiction.
 Qed.
 Next Obligation.
-  intros ? ? ? ? ? ? ? ? ? ? ? nb Hstep ; simpl in *.
+  intros ? ? ? ? ? ? ? ? ? ? nb Hstep ; simpl in *.
   inversion Hstep; subst; simpl in *.
   - apply (lts_oba_mo_spec2 a1 η a2) in nb; eauto. multiset_solver.
   - apply (non_blocking_action_in_ms b1 η b2) in nb as eq; eauto; subst.
@@ -644,7 +644,7 @@ Next Obligation.
     eapply lts_mb_nb_spec1;eauto.
 Qed.
 Next Obligation.
-intros ? ? ? ? ? ? ? ? ? ? ? ? ? nb Hstep_nb Hstep. destruct p as (p, mp), q as (q, mq), r as (r, mr).
+intros ? ? ? ? ? ? ? ? ? ? ? ? nb Hstep_nb Hstep. destruct p as (p, mp), q as (q, mq), r as (r, mr).
   inversion Hstep_nb; inversion Hstep; subst.
   - destruct (lts_oba_non_blocking_action_delay nb l l0) as (t & hlt0 & (r0 & hlr0 & heqr0)).
     exists (t, mr). split; simpl in *. eauto with mdb.
@@ -688,7 +688,7 @@ intros ? ? ? ? ? ? ? ? ? ? ? ? ? nb Hstep_nb Hstep. destruct p as (p, mp), q as 
     + exists (r ▷ mr). split. eapply ParRight. apply lts_multiset_minus; exact nb. reflexivity.
 Qed.
 Next Obligation.
-  intros ? ? ? ? ? ? ? ? ? ? ? ? ? nb not_eq Hstep_nb Hstep. 
+  intros ? ? ? ? ? ? ? ? ? ? ? ? nb not_eq Hstep_nb Hstep. 
   destruct p as (p, mp), q1 as (q, mq), q2 as (r, mr).
   inversion Hstep_nb; subst.
   - inversion Hstep; subst.
@@ -723,7 +723,7 @@ Next Obligation.
 Qed.
 Next Obligation.
 Proof.
-  intros ? ? ? ? ? ? ? ? (p1, m1) (p2, m2) (p3, m3) η nb Hstep_nb Hstep.
+  intros ? ? ? ? ? ? ? (p1, m1) (p2, m2) (p3, m3) η nb Hstep_nb Hstep.
   inversion Hstep_nb ;subst.
   - inversion Hstep ; subst.
     + edestruct (lts_oba_non_blocking_action_tau nb l l0) as
@@ -767,7 +767,7 @@ Proof.
          eapply ParRight. eapply lts_multiset_minus; eauto. reflexivity.
 Qed.
 Next Obligation.
-  intros ? ? ? ? ? ? ? ? (p1, m1) (p2, m2) (p3, m3) η nb Hstep_nb Hstep_nb'.
+  intros ? ? ? ? ? ? ? (p1, m1) (p2, m2) (p3, m3) η nb Hstep_nb Hstep_nb'.
   intros p2' p3' hwp2 hwp3; simpl in *.
   inversion Hstep_nb ; subst.
   - inversion Hstep_nb' ; subst.
@@ -803,7 +803,7 @@ Next Obligation.
       split.  eapply strip_m_deter; eauto. multiset_solver.
 Qed.
 Next Obligation.
-  intros ? ? ? ? ? ? ? ? (p1, mp1) (p2, mp2) (q1, mq1) (q2, mq2) η nb Hstep_nb Hstep_nb' equiv.
+  intros ? ? ? ? ? ? ? (p1, mp1) (p2, mp2) (q1, mq1) (q2, mq2) η nb Hstep_nb Hstep_nb' equiv.
   inversion Hstep_nb; subst;  intros p1' p2' hwp1 hwp2; simpl in *.
   - eapply lts_oba_mo_spec2 in l as hd1; eauto.
     edestruct (lts_oba_mo_strip q1) as (q1' & hwq1).
@@ -870,17 +870,17 @@ Qed.
 (* Forwarder of a LTS with OBA axioms respects FW axioms *)
 
 #[global] Program Instance FW_gLtsObaFW
-  `{M : @gLtsObaFB P A H gLtsP gLtsEqP gLtsObaP}
-  `{@Prop_of_Inter P (mb A) A fw_inter H gLtsP MbgLts}
+  `{M : @gLtsObaFB P A H gLtsEqP gLtsObaP}
+   `{!Prop_of_Inter P (mb A) A fw_inter}
   : gLtsObaFW (P * mb A) A.
 Next Obligation.
-  intros ? ? ? ? ? ? ? ? (p, m) η μ.
+  intros ? ? ? ? ? ? ? (p, m) η μ.
   exists (p, {[+ η +]} ⊎ m). split; eauto with mdb.
   eapply ParRight. eapply lts_multiset_add; eauto.
   eapply ParRight. eapply lts_multiset_minus; eauto.
 Qed.
 Next Obligation.
-  intros ? ? ? ? ? ? ? ? (p1, m1) (p2, m2) (p3, m3) η μ nb duo Hstep_nb Hstep.
+  intros ? ? ? ? ? ? ? (p1, m1) (p2, m2) (p3, m3) η μ nb duo Hstep_nb Hstep.
   inversion Hstep_nb; subst.
   + inversion Hstep; subst.
     ++ left. destruct (lts_oba_fb_feedback nb duo l l0) as (t & l1 & heq).
