theories/Interaction_Between_Lts/InteractionBetweenLts.v
@@ -28,7 +28,7 @@ From Coq.Unicode Require Import Utf8.
 From Coq.Lists Require Import List.
 Import ListNotations.
 From Coq.Wellfounded Require Import Inverse_Image.
-
+From Coq.Logic Require Import JMeq ProofIrrelevance.
 From Coq.Program Require Import Wf Equality.
 From stdpp Require Import base countable list decidable finite gmap gmultiset.
 From Must Require Import ForAllHelper MultisetHelper gLts Bisimulation Lts_OBA Lts_FW FiniteImageLTS 
@@ -834,7 +834,7 @@ Definition inter_lts_refuses `{Prop_of_Inter S1 S2 A}
 #[global] Instance inter_lts 
   `(inter : A -> A -> Prop)
   `{Prop_of_Inter S1 S2 A inter} :
-  gLts (S1 * S2) A. 
+  gLts (S1 * S2) _.
 Proof.
   refine (MkgLts _ _ _ inter_step _ _ (λ s, inter_lts_refuses s.1 s.2) _ _ _).
   - intros [s1 s2] ℓ [s'1 s'2]. apply decide_inter_step.
@@ -867,7 +867,7 @@ Proof.
 Defined.
 
 #[global]
-Instance inter_clts {S1 S2 A: Type} `{H : ExtAction A}  `{!gLts S1 A} `{!gLts S2 A} 
+Instance inter_clts {S1 S2 A: Type} `{H : ExtAction A}  `{!gLts S1 H} `{!gLts S2 H} 
 `{M1: !CountablegLts S1 A} 
 `{M2: !CountablegLts S2 A} `{inter : A -> A -> Prop} 
 `{i : !Prop_of_Inter S1 S2 A inter}: CountablegLts (S1 * S2) A.
