theories/Testing_Pre_orders/May/LiftMay.v
@@ -32,10 +32,10 @@ From Must Require Import ForAllHelper gLts Bisimulation Lts_OBA Lts_OBA_FB Lts_F
 From Must Require Import ActTau.
 
 Lemma may_non_blocking_action_swap_l_fw_eq `{
-  @gLtsObaFW P A H gLtsP gLtsEqP gLtsObaP, 
-  @gLtsObaFB T A H gLtsT gLtsEqT gLtsObaT, !Testing_Predicate T A outcome}
+   @gLtsObaFW P A H gLtsEqP gLtsObaP, 
+  !@gLtsObaFB T A H gLtsEqT gLtsObaT, !Testing_Predicate T A outcome}
 
-  `{@Prop_of_Inter P T A parallel_inter H gLtsP gLtsT}
+  {_ : Prop_of_Inter P T A dual}
 
   (p1 p2 : P) (t1 t2 : T) (η : A) :
   non_blocking η -> p1 ⟶⋍[η] p2 -> t1 ⟶⋍[η] t2 -> p1 may_pass t2
@@ -45,10 +45,10 @@ Proof.
 Admitted.
 
 Lemma may_non_blocking_action_swap_r_fw_eq`{
-  @gLtsObaFW P A H gLtsP gLtsEqP gLtsObaP, 
-  @gLtsObaFB T A H gLtsT gLtsEqT gLtsObaT, !Testing_Predicate T A outcome}
+  @gLtsObaFW P A H gLtsEqP gLtsObaP, 
+  @gLtsObaFB T A H gLtsEqT gLtsObaT, !Testing_Predicate T A outcome}
 
-  `{@Prop_of_Inter P T A parallel_inter H gLtsP gLtsT}
+  {_ : Prop_of_Inter P T A dual}
 
   (p1 p2 : P) (t1 t2 : T) (η : A) :
   non_blocking η -> p1 ⟶⋍[η] p2 -> t1 ⟶⋍[η] t2 -> p2 may_pass t1
@@ -58,10 +58,10 @@ Proof.
 Admitted.
 
 Lemma may_non_blocking_action_swap_l_fw `{
-  @gLtsObaFW P A H gLtsP gLtsEqP gLtsObaP, 
-  @gLtsObaFB T A H gLtsT gLtsEqT gLtsObaT, !Testing_Predicate T A outcome}
+  @gLtsObaFW P A H gLtsEqP gLtsObaP, 
+  @gLtsObaFB T A H gLtsEqT gLtsObaT, !Testing_Predicate T A outcome}
 
-  `{@Prop_of_Inter P T A parallel_inter H gLtsP gLtsT}
+  {_ : Prop_of_Inter P T A dual}
 
   (p1 p2 : P) (t1 t2 : T) (η : A) :
   non_blocking η -> p1 ⟶[η] p2 -> t1 ⟶[η] t2 -> p1 may_pass t2 
@@ -71,10 +71,10 @@ Proof.
 Qed.
 
 Lemma may_non_blocking_action_swap_r_fw `{
-  @gLtsObaFW P A H gLtsP gLtsEqP gLtsObaP, 
-  @gLtsObaFB T A H gLtsT gLtsEqT gLtsObaT, !Testing_Predicate T A outcome}
+  @gLtsObaFW P A H gLtsEqP gLtsObaP, 
+  @gLtsObaFB T A H gLtsEqT gLtsObaT, !Testing_Predicate T A outcome}
 
-  `{@Prop_of_Inter P T A parallel_inter H gLtsP gLtsT}
+  {_ : Prop_of_Inter P T A dual}
 
   (p1 p2 : P) (t1 t2 : T) (η : A) :
   non_blocking η -> p1 ⟶[η] p2 -> t1 ⟶[η] t2 -> may p2 t1
@@ -85,11 +85,11 @@ Proof.
 Qed.
 
 Lemma nf_may_fw_l `{
-  @gLtsObaFB P A H gLtsP gLtsEqP gLtsObaP, !FiniteImagegLts P A,
-  @gLtsObaFB T A H gLtsT gLtsEqT gLtsObaT, !Testing_Predicate T A outcome}
+  @gLtsObaFB P A H gLtsEqP gLtsObaP, !FiniteImagegLts P A,
+  @gLtsObaFB T A H gLtsEqT gLtsObaT, !Testing_Predicate T A outcome}
 
-  `{@Prop_of_Inter P (mb A) A fw_inter H gLtsP MbgLts}
-  `{@Prop_of_Inter (P * mb A) T A parallel_inter H (inter_lts fw_inter) gLtsT}
+  {_ : Prop_of_Inter P (mb A) A fw_inter}
+  {_ : Prop_of_Inter (P * mb A) T A dual}
 
   m1 m2 (p : P) (t t' : T) : t ⟿{m1} t' -> (p, m1 ⊎ m2) may_pass t' -> (p, m2) may_pass t.
 Proof.
@@ -114,11 +114,11 @@ Proof.
 Qed.
 
 Lemma nf_may_fw_r `{
-  @gLtsObaFB P A H gLtsP gLtsEqP gLtsObaP, !FiniteImagegLts P A ,
-  @gLtsObaFB T A H gLtsT gLtsEqT gLtsObaT, !Testing_Predicate T A outcome}
+  @gLtsObaFB P A H gLtsEqP gLtsObaP, !FiniteImagegLts P A ,
+  @gLtsObaFB T A H gLtsEqT gLtsObaT, !Testing_Predicate T A outcome}
 
-  `{@Prop_of_Inter P (mb A) A fw_inter H gLtsP MbgLts}
-  `{@Prop_of_Inter (P * mb A) T A parallel_inter H (inter_lts fw_inter) gLtsT}
+  {_ : Prop_of_Inter P (mb A) A fw_inter}
+  {_ : Prop_of_Inter (P * mb A) T A dual}
 
   (p : P) (t t' : T) m1 m2 : 
   t ⟿{m1} t' -> (p, m2) may_pass t -> (p, m1 ⊎ m2) may_pass t'.
@@ -134,11 +134,11 @@ Proof.
 Admitted.
 
 Lemma nf_may_fw `{
-  @gLtsObaFB P A H gLtsP gLtsEqP gLtsObaP, !FiniteImagegLts P A ,
-  @gLtsObaFB T A H gLtsT gLtsEqT gLtsObaT, !Testing_Predicate T A outcome}
+  @gLtsObaFB P A H gLtsEqP gLtsObaP, !FiniteImagegLts P A ,
+  @gLtsObaFB T A H gLtsEqT gLtsObaT, !Testing_Predicate T A outcome}
 
-  `{@Prop_of_Inter P (mb A) A fw_inter H gLtsP MbgLts}
-  `{@Prop_of_Inter (P * mb A) T A parallel_inter H (inter_lts fw_inter) gLtsT}
+  {_ : Prop_of_Inter P (mb A) A fw_inter}
+  {_ : Prop_of_Inter (P * mb A) T A dual}
 
   (p : P) (t t' : T) m : 
   t ⟿{m} t' -> (p, m) may_pass t' <-> (p, ∅) may_pass t.
@@ -149,12 +149,12 @@ Proof.
 Qed.
 
 Lemma may_to_may_fw `{
-  @gLtsObaFB P A H gLtsP gLtsEqP gLtsObaP, !FiniteImagegLts P A,
-  @gLtsObaFB T A H gLtsT gLtsEqT gLtsObaT, !Testing_Predicate T A outcome}
+  @gLtsObaFB P A H gLtsEqP gLtsObaP, !FiniteImagegLts P A,
+  @gLtsObaFB T A H gLtsEqT gLtsObaT, !Testing_Predicate T A outcome}
 
-  `{@Prop_of_Inter P (mb A) A fw_inter H gLtsP MbgLts}
-  `{@Prop_of_Inter (P * mb A) T A parallel_inter H (inter_lts fw_inter) gLtsT}
-  `{@Prop_of_Inter P T A parallel_inter H gLtsP gLtsT}
+  {_ : Prop_of_Inter P (mb A) A fw_inter}
+  {_ : Prop_of_Inter (P * mb A) T A dual}
+  {_ : Prop_of_Inter P T A dual}
 
   (p : P) (t : T) (m : mb A) :
   p may_pass t -> m = lts_oba_mo t -> forall t', t ⟿{m} t' 
@@ -169,12 +169,12 @@ Proof.
 Admitted.
 
 Lemma may_fw_to_may `{
-  @gLtsObaFB P A H gLtsP gLtsEqP gLtsObaP, !FiniteImagegLts P A,
-  @gLtsObaFB T A H gLtsT gLtsEqT gLtsObaT, !Testing_Predicate T A outcome}
+  @gLtsObaFB P A H gLtsEqP gLtsObaP, !FiniteImagegLts P A,
+  @gLtsObaFB T A H gLtsEqT gLtsObaT, !Testing_Predicate T A outcome}
 
-  `{@Prop_of_Inter P (mb A) A fw_inter H gLtsP MbgLts}
-  `{@Prop_of_Inter (P * mb A) T A parallel_inter H (inter_lts fw_inter) gLtsT}
-  `{@Prop_of_Inter P T A parallel_inter H gLtsP gLtsT}
+  {_ : Prop_of_Inter P (mb A) A fw_inter}
+  {_ : Prop_of_Inter (P * mb A) T A dual}
+  {_ : Prop_of_Inter P T A dual}
 
   (p : P) (t : T) :
   (p, ∅) may_pass t -> p may_pass t.
@@ -187,12 +187,12 @@ Proof.
 Admitted.
 
 Lemma may_iff_may_fw `{
-  @gLtsObaFB P A H gLtsP gLtsEqP gLtsObaP, !FiniteImagegLts P A,
-  @gLtsObaFB T A H gLtsT gLtsEqT gLtsObaT, !Testing_Predicate T A outcome}
+  @gLtsObaFB P A H gLtsEqP gLtsObaP, !FiniteImagegLts P A,
+  @gLtsObaFB T A H gLtsEqT gLtsObaT, !Testing_Predicate T A outcome}
 
-  `{@Prop_of_Inter P (mb A) A fw_inter H gLtsP MbgLts}
-  `{@Prop_of_Inter (P * mb A) T A parallel_inter H (inter_lts fw_inter) gLtsT}
-  `{@Prop_of_Inter P T A parallel_inter H gLtsP gLtsT}
+  {_ : Prop_of_Inter P (mb A) A fw_inter}
+  {_ : Prop_of_Inter (P * mb A) T A dual}
+  {_ : Prop_of_Inter P T A dual}
 
   (p : P) (t : T) :
   p may_pass t <-> (p, ∅) may_pass t.
@@ -206,21 +206,19 @@ Proof.
 Qed.
 
 Lemma lift_fw_ctx_pre `{
-    @gLtsObaFB P A H gLtsP gLtsEqP gLtsObaP, !FiniteImagegLts P A,
-    @gLtsObaFB Q A H gLtsQ gLtsEqQ gLtsObaQ, !FiniteImagegLts Q A,
-    @gLtsObaFB T A H gLtsT gLtsEqT gLtsObaT, !Testing_Predicate T A outcome}
+    @gLtsObaFB P A H gLtsEqP gLtsObaP, !FiniteImagegLts P A,
+    @gLtsObaFB Q A H gLtsEqQ gLtsObaQ, !FiniteImagegLts Q A,
+    @gLtsObaFB T A H gLtsEqT gLtsObaT, !Testing_Predicate T A outcome}
 
-  `{@Prop_of_Inter P (mb A) A fw_inter H gLtsP MbgLts}
+  {_ : Prop_of_Inter P (mb A) A fw_inter}
+  {_ : Prop_of_Inter (P * mb A) T A dual}
 
-  `{@Prop_of_Inter (P * mb A) T A parallel_inter H (inter_lts fw_inter) gLtsT}
+  {_ : Prop_of_Inter P T A dual}
 
-  `{@Prop_of_Inter P T A parallel_inter H gLtsP gLtsT}
+  {_ : Prop_of_Inter Q (mb A) A fw_inter}
+  {_ : Prop_of_Inter (Q * mb A) T A dual}
 
-  `{@Prop_of_Inter Q (mb A) A fw_inter H gLtsQ MbgLts}
-
-  `{@Prop_of_Inter (Q * mb A) T A parallel_inter H (inter_lts fw_inter) gLtsT}
-
-  `{@Prop_of_Inter Q T A parallel_inter H gLtsQ gLtsT}
+  {_ : Prop_of_Inter Q T A dual}
 
   (p : P) (q : Q) : p ⊑ₘₐᵧ q <-> (p, ∅) ⊑ₘₐᵧ (q, ∅).
 Proof.
